Almost final version of paper

KAT_Module.thy
@@ -13,10 +13,10 @@ end
 locale kat_module' =
   fixes K :: "'a test_algebra"
   and A :: "('b, 'c) ord_scheme"
-  and mk :: "'a \<Rightarrow> 'b \<Rightarrow> 'b"
+  and scalar_product :: "'b \<Rightarrow> 'a \<Rightarrow> 'b"
   assumes kat_subalg: "kat K"
   and cbl_subalg: "complete_boolean_lattice A"
-  and mk_type: "mk : carrier K \<rightarrow> carrier A \<rightarrow> carrier A"
+  and mk_type: "scalar_product : carrier A \<rightarrow> carrier K \<rightarrow> carrier A"
 
 sublocale kat_module' \<subseteq> kat K using kat_subalg .
 sublocale kat_module' \<subseteq> A: complete_boolean_lattice A using cbl_subalg .
@@ -45,7 +45,7 @@ begin
   abbreviation zero :: "'a" ("0") where "0 \<equiv> Dioid.zero K"
 
   abbreviation module :: "'b \<Rightarrow> 'a \<Rightarrow> 'b" (infixl "\<Colon>" 75) where
-    "m \<Colon> p \<equiv> mk p m"
+    "m \<Colon> p \<equiv> scalar_product m p"
 
   abbreviation star :: "'a \<Rightarrow> 'a" ("_\<^sup>\<star>" [101] 100) where
     "x\<^sup>\<star> \<equiv> Kleene_Algebra.star K x"
@@ -99,11 +99,6 @@ begin
     finally show ?thesis .
   qed
 
-      (*
-  lemma mod_star2: "\<lbrakk>m \<in> carrier A; p \<in> carrier K; q \<in> carrier K\<rbrakk> \<Longrightarrow> m \<Colon> (p + q) \<sqsubseteq>\<^bsub>A\<^esub> m \<Longrightarrow> m \<Colon> p\<^sup>\<star> \<sqsubseteq>\<^bsub>A\<^esub> m"
-    by (metis (lifting) A.bot_closed bot_oner mod_bot mod_join mod_zero prop_bot star_closed zero_closed)
-      *)
-
   lemma mod_closed [intro]: "\<lbrakk>p \<in> carrier K; P \<in> carrier A\<rbrakk> \<Longrightarrow> P \<Colon> p \<in> carrier A"
     by (metis mk_type typed_application)
 
@@ -119,32 +114,32 @@ begin
   lemma mod_zero_bot: "\<lbrakk>p \<in> carrier K; M \<in> carrier A; p \<preceq> 0\<rbrakk> \<Longrightarrow> M \<Colon> p \<sqsubseteq>\<^bsub>A\<^esub> \<bottom>"
     by (subgoal_tac "p = 0", auto simp add: mod_zero) (metis add_zeror nat_order_def)
 
-  definition hoare_triple :: "'b \<Rightarrow> 'a \<Rightarrow> 'b \<Rightarrow> bool" ("_ \<lbrace> _ \<rbrace> _" [54,54,54] 53) where
-    "P \<lbrace> p \<rbrace> Q \<equiv> P \<Colon> p \<sqsubseteq>\<^bsub>A\<^esub> Q"
+  definition hoare_triple :: "'b \<Rightarrow> 'a \<Rightarrow> 'b \<Rightarrow> bool" ("\<lbrace>_\<rbrace> _ \<lbrace>_\<rbrace>" [54,54,54] 53) where
+    "\<lbrace>P\<rbrace> p \<lbrace>Q\<rbrace> \<equiv> P \<Colon> p \<sqsubseteq>\<^bsub>A\<^esub> Q"
 
   lemma hoare_composition:
     assumes pc: "p \<in> carrier K" and qc: "q \<in> carrier K"
     and Pc: "P \<in> carrier A" and Qc: "Q \<in> carrier A" and Rc: "R \<in> carrier A"
-    and p_triple: "P \<lbrace>p\<rbrace> Q" and q_triple: "Q \<lbrace>q\<rbrace> R"
-    shows "P \<lbrace>p \<cdot> q\<rbrace> R"
+    and p_triple: "\<lbrace>P\<rbrace> p \<lbrace>Q\<rbrace>" and q_triple: "\<lbrace>Q\<rbrace> q \<lbrace>R\<rbrace>"
+    shows "\<lbrace>P\<rbrace> p \<cdot> q \<lbrace>R\<rbrace>"
     by (smt A.join_assoc A.leq_def Pc Qc Rc hoare_triple_def mod_closed mod_join mod_mult p_triple pc q_triple qc)
 
-  lemma hoare_skip: shows "P \<in> carrier A \<Longrightarrow> P \<lbrace> 1 \<rbrace> P"
+  lemma hoare_skip: shows "P \<in> carrier A \<Longrightarrow> \<lbrace>P\<rbrace> 1 \<lbrace>P\<rbrace>"
     by (metis A.order_refl hoare_triple_def mod_one)
 
   lemma hoare_weakening:
     assumes Pc[intro]: "P \<in> carrier A" and P'c[intro]: "P' \<in> carrier A"
     and Qc[intro]: "Q \<in> carrier A" and Q'c[intro]: "Q' \<in> carrier A"
     and pc[intro]: "p \<in> carrier K"
-    shows "\<lbrakk>P \<lbrace> p \<rbrace> Q; P' \<sqsubseteq>\<^bsub>A\<^esub> P; Q \<sqsubseteq>\<^bsub>A\<^esub> Q'\<rbrakk> \<Longrightarrow> P' \<lbrace> p \<rbrace> Q'"
+    shows "\<lbrakk>\<lbrace>P\<rbrace> p \<lbrace>Q\<rbrace>; P' \<sqsubseteq>\<^bsub>A\<^esub> P; Q \<sqsubseteq>\<^bsub>A\<^esub> Q'\<rbrakk> \<Longrightarrow> \<lbrace>P'\<rbrace> p \<lbrace>Q'\<rbrace>"
   proof -
     assume "Q \<sqsubseteq>\<^bsub>A\<^esub> Q'"
-    hence a: "Q \<lbrace> 1 \<rbrace> Q'"
+    hence a: "\<lbrace>Q\<rbrace> 1 \<lbrace>Q'\<rbrace>"
       by (metis Qc hoare_triple_def mod_one)
-    assume "P \<lbrace> p \<rbrace> Q" and "P' \<sqsubseteq>\<^bsub>A\<^esub> P"
-    hence b: "P' \<lbrace> p \<rbrace> Q"
+    assume "\<lbrace>P\<rbrace> p \<lbrace>Q\<rbrace>" and "P' \<sqsubseteq>\<^bsub>A\<^esub> P"
+    hence b: "\<lbrace>P'\<rbrace> p \<lbrace>Q\<rbrace>"
       by (simp add: hoare_triple_def, rule_tac y = "P \<Colon> p" in A.order_trans) (metis P'c Pc mod_A_iso pc, auto)
-    have "P' \<lbrace> p \<cdot> 1 \<rbrace> Q'"
+    have "\<lbrace>P'\<rbrace> p \<cdot> 1 \<lbrace>Q'\<rbrace>"
       by (metis (lifting) P'c Q'c Qc a b hoare_composition one_closed pc)
     thus ?thesis
       by (metis mult_oner pc)
@@ -155,9 +150,9 @@ begin
   lemma hoare_plus:
     assumes pc [intro]: "p \<in> carrier K" and qc [intro]: "q \<in> carrier K"
     and Pc [intro]: "P \<in> carrier A" and Qc [intro]: "Q \<in> carrier A"
-    and then_branch: "P \<lbrace> p \<rbrace> Q"
-    and else_branch: "P \<lbrace> q \<rbrace> Q"
-    shows "P \<lbrace> p + q \<rbrace> Q"
+    and then_branch: "\<lbrace>P\<rbrace> p \<lbrace>Q\<rbrace>"
+    and else_branch: "\<lbrace>P\<rbrace> q \<lbrace>Q\<rbrace>"
+    shows "\<lbrace>P\<rbrace> p + q \<lbrace>Q\<rbrace>"
   proof -
     have "P \<Colon> p \<sqsubseteq>\<^bsub>A\<^esub> Q" and "P \<Colon> q \<sqsubseteq>\<^bsub>A\<^esub> Q"
       by (insert then_branch else_branch) (simp add: hoare_triple_def)+
@@ -173,9 +168,9 @@ begin
     assumes b_test: "b \<in> tests K"
     and pc: "p \<in> carrier K" and qc: "q \<in> carrier K"
     and Pc: "P \<in> carrier A" and Qc: "Q \<in> carrier A"
-    and then_branch: "P \<sqinter> (\<top> \<Colon> b) \<lbrace> p \<rbrace> Q"
-    and else_branch: "P \<sqinter> (\<top> \<Colon> !b) \<lbrace> q \<rbrace> Q"
-    shows "P \<lbrace> b\<cdot>p + !b\<cdot>q \<rbrace> Q"
+    and then_branch: "\<lbrace>P \<sqinter> (\<top> \<Colon> b)\<rbrace> p \<lbrace>Q\<rbrace>"
+    and else_branch: "\<lbrace>P \<sqinter> (\<top> \<Colon> !b)\<rbrace> q \<lbrace>Q\<rbrace>"
+    shows "\<lbrace>P\<rbrace> b\<cdot>p + !b\<cdot>q \<lbrace>Q\<rbrace>"
     apply (rule hoare_plus)
     apply (metis (lifting) b_test mult_closed pc test_subset_var)
     apply (metis b_test local.complement_closed mult_closed qc test_subset_var)
@@ -201,8 +196,8 @@ begin
   lemma hoare_star:
     assumes pc: "p \<in> carrier K"
     and Pc: "P \<in> carrier A"
-    and p_triple: "P \<lbrace> p \<rbrace> P"
-    shows "P \<lbrace> p\<^sup>\<star> \<rbrace> P"
+    and p_triple: "\<lbrace>P\<rbrace> p \<lbrace>P\<rbrace>"
+    shows "\<lbrace>P\<rbrace> p\<^sup>\<star> \<lbrace>P\<rbrace>"
     by (metis (lifting) A.bin_lub_var A.order_refl Pc hoare_triple_def mod_closed mod_star p_triple pc)
 
   declare star_closed [intro]
@@ -212,20 +207,42 @@ begin
   declare meet_closed [intro!]
   declare top_closed [intro]
 
-  lemma [intro]: "\<lbrakk>b \<in> tests K; P \<in> carrier A\<rbrakk> \<Longrightarrow> P \<lbrace> b \<rbrace> P \<sqinter>\<^bsub>A\<^esub> \<top> \<Colon> b"
+  lemma [intro]: "\<lbrakk>b \<in> tests K; P \<in> carrier A\<rbrakk> \<Longrightarrow> \<lbrace>P\<rbrace> b \<lbrace>P \<sqinter>\<^bsub>A\<^esub> \<top> \<Colon> b\<rbrace>"
     by (metis A.eq_refl hoare_triple_def mod_closed mod_test test_subset_var)
 
-   lemma hoare_while:
+  lemma hoare_while:
     assumes b_test [intro]: "b \<in> tests K" and pc [intro]: "p \<in> carrier K"
     and Pc [intro]: "P \<in> carrier A"
-    and loop_condition [intro]: "P \<sqinter> (\<top> \<Colon> b) \<lbrace>p\<rbrace> P"
-    shows "P \<lbrace> (b\<cdot>p)\<^sup>\<star>\<cdot>!b \<rbrace> P \<sqinter> (\<top> \<Colon> !b)"
+    and loop_condition [intro]: "\<lbrace>P \<sqinter> (\<top> \<Colon> b)\<rbrace> p \<lbrace>P\<rbrace>"
+    shows "\<lbrace>P\<rbrace> (b\<cdot>p)\<^sup>\<star>\<cdot>!b \<lbrace>P \<sqinter> (\<top> \<Colon> !b)\<rbrace>"
   proof (rule hoare_composition[where ?Q = P], auto)
-    show "P \<lbrace> (b \<cdot> p)\<^sup>\<star> \<rbrace> P"
+    show "\<lbrace>P\<rbrace> (b \<cdot> p)\<^sup>\<star> \<lbrace>P\<rbrace>"
       by (blast intro: hoare_star hoare_composition[where ?Q = "P \<sqinter> \<top> \<Colon> b"])
   qed
 
+lemma derived_rule1:
+  assumes p: "{P1,P2,Q1,Q2} \<subseteq> carrier A" and q: "p \<in> carrier K"
+  and "\<lbrace>P1\<rbrace> p \<lbrace>Q1\<rbrace>" and "\<lbrace>P2\<rbrace> p \<lbrace>Q2\<rbrace>"
+  shows "\<lbrace>P1 \<sqinter> P2\<rbrace> p \<lbrace>Q1 \<sqinter> Q2\<rbrace>"
+  using assms
+  apply (auto intro: simp add: hoare_triple_def assms, subst A.bin_glb_var)
+  by (metis A.absorb1 A.bin_lub_var A.meet_closed A.meet_comm mod_closed mod_join)+
+
+lemma derived_rule2:
+  assumes "P \<in> carrier A" and "p \<in> carrier K" and "P \<Colon> p = (\<top> \<Colon> p) \<sqinter> P"
+  shows "\<lbrace>P\<rbrace> p \<lbrace>P\<rbrace>"
+  using assms
+  by (metis (lifting) A.bin_glb_var A.eq_refl A.top_closed hoare_triple_def mod_closed)
+
+lemma derived_rule3:
+  assumes "{P,Q,R} \<subseteq> carrier A" and "p \<in> carrier K" and "P \<Colon> p = (\<top> \<Colon> p) \<sqinter> P"
+  and "\<lbrace>Q\<rbrace> p \<lbrace>R\<rbrace>"
+  shows "\<lbrace>P \<sqinter> Q\<rbrace> p \<lbrace>P \<sqinter> R\<rbrace>"
+  by (insert assms) (smt derived_rule1 derived_rule2 insert_subset)
+
 end
+
+lemma "range f = (\<Union>x. {f x})" and "(\<Union>x. {f x}) = {f i|i. True}" by auto
 
 end
 
